MonadClass/MonadAlt2.v
@@ -1,0 +1,16 @@
+Require Import HSLib.Base.
+Require Import Control.Monad.
+Require Import Control.Alternative.
+Require Import Control.Foldable.
+
+Class MonadAlt (M : Type -> Type) (inst : Monad M) : Type :=
+{
+    choose : forall {A : Type}, M A -> M A -> M A;
+    choose_assoc :
+      forall {X : Type} (a b c : M X),
+        choose (choose a b) c = choose a (choose b c);
+    choose_bind_r :
+      forall (A B : Type) (m : M A) (f g : A -> M B),
+        (m >>= fun x : A => choose (f x) (g x)) =
+        choose (m >>= f) (m >>= g)
+}.
