MonadClass/MonadAltBag.v
@@ -1,0 +1,15 @@
+Require Import HSLib.Base.
+Require Import Control.Monad.
+
+(** The initial model are finite bags
+    (which probably means finite multisets). *)
+Class MonadAltBag (M : Type -> Type) (inst : Monad M) : Type :=
+{
+    choose : forall {A : Type}, M A -> M A -> M A;
+    choose_assoc :
+      forall {X : Type} (a b c : M X),
+        choose (choose a b) c = choose a (choose b c);
+    choose_comm :
+      forall {A : Type} (x y : M A),
+        choose x y = choose y x
+}.
