MonadClass/MonadNondet.v
@@ -1,0 +1,17 @@
+Require Import HSLib.Base.
+Require Import Control.Monad.
+
+Require Import MonadClass.MonadFail.
+Require Import MonadClass.MonadAlt.
+
+Class MonadNondet (M : Type -> Type) (inst : Monad M) : Type :=
+{
+    instF :> MonadFail;
+    instA :> MonadAlt;
+    choose_fail_l :
+      forall (A : Type) (x : M A),
+        choose fail x = x;
+    choose_fail_r :
+      forall (A : Type) (x : M A),
+        choose x fail = x;
+}.
